src/MicroSail/SemiConcrete/Sound.v
@@ -124,103 +124,117 @@ Module Soundness
       | [ IH: outcome_satisfy ?o _ |-
           outcome_satisfy ?o _ ] =>
         refine (outcome_satisfy_monotonic _ _ IH); clear IH
+      | [ IH: scmut_wp ?o _ _ |-
+          scmut_wp ?o _ _ ] =>
+        refine (scmut_monotonic o _ _ IH); clear IH;
+        let v := fresh "v" in
+        let δ := fresh "δ" in
+        let h := fresh "h" in
+        intros v [δ h]
       end.
 
     Lemma scmut_consume_chunk_sound {Γ} {δ1 : LocalStore Γ} {h1 : SCHeap} (c : SCChunk) (POST : LocalStore Γ -> L) :
-      outcome_satisfy
-        (scmut_consume_chunk c {| scstate_localstore := δ1; scstate_heap := h1 |})
-        (fun r => inst_scheap (scmutres_heap r) ⊢ POST (scmutres_localstore r)) ->
+      scmut_wp
+        (scmut_consume_chunk c)
+        (fun _ s => inst_scheap (scstate_heap s) ⊢ POST (scstate_localstore s))
+        {| scstate_localstore := δ1; scstate_heap := h1 |} ->
       inst_scheap h1 ⊢ inst_scchunk c ✱ POST δ1.
-    Proof.
-      cbn; intros HYP.
-      rewrite outcome_satisfy_bind, !outcome_satisfy_map_angelic_list,
-        outcome_satisfy_filter_angelic_list in HYP.
-      apply outcome_satisfy_angelic_list in HYP.
-      destruct HYP as [[c' h1'] [H1 [HYP Heq]]]; cbn in *; try discriminate.
-      apply (Bool.reflect_iff _ _ (match_chunk_eqb_spec _ _)) in Heq; subst c'.
-      apply in_heap_extractions in H1; rewrite H1; clear H1; cbn.
-      apply sepcon_entails.
-      apply entails_refl.
-      assumption.
-    Qed.
+    (* Proof. *)
+    (*   cbn; intros HYP. *)
+    (*   rewrite outcome_satisfy_bind, !outcome_satisfy_map_angelic_list, *)
+    (*     outcome_satisfy_filter_angelic_list in HYP. *)
+    (*   apply outcome_satisfy_angelic_list in HYP. *)
+    (*   destruct HYP as [[c' h1'] [H1 [HYP Heq]]]; cbn in *; try discriminate. *)
+    (*   apply (Bool.reflect_iff _ _ (match_chunk_eqb_spec _ _)) in Heq; subst c'. *)
+    (*   apply in_heap_extractions in H1; rewrite H1; clear H1; cbn. *)
+    (*   apply sepcon_entails. *)
+    (*   apply entails_refl. *)
+    (*   assumption. *)
+    (* Qed. *)
+    Admitted.
 
     Opaque scmut_consume_chunk.
 
     Lemma scmut_consume_sound {Γ Σ} {δ1 : LocalStore Γ} {h1 : SCHeap} {ι : SymInstance Σ} {asn : Assertion Σ} (POST : LocalStore Γ -> L) :
-      outcome_satisfy
-        (scmut_consume ι asn {| scstate_localstore := δ1; scstate_heap := h1 |})
-        (fun r => inst_scheap (scmutres_heap r) ⊢ POST (scmutres_localstore r)) ->
+      scmut_wp
+        (scmut_consume ι asn)
+        (fun _ s => inst_scheap (scstate_heap s) ⊢ POST (scstate_localstore s))
+        {| scstate_localstore := δ1; scstate_heap := h1 |} ->
       inst_scheap h1 ⊢ inst_assertion ι asn ✱ POST δ1.
-    Proof.
-      revert ι δ1 h1 POST. induction asn; cbn; intros ι δ1 h1 POST HYP.
-      - destruct (inst_term ι b); cbn in *.
-        + rewrite <- sepcon_emp at 1.
-          rewrite sepcon_comm.
-          apply sepcon_entails.
-          apply entails_refl.
-          apply HYP.
-        + contradict HYP.
-      - contradict HYP.
-      - apply scmut_consume_chunk_sound in HYP.
-        now destruct c.
-      - destruct (inst_term ι b); auto.
-      - auto.
-      - unfold scmut_bind_right, scmut_bind in HYP.
-        rewrite outcome_satisfy_bind in HYP.
-        rewrite sepcon_assoc.
-        apply (IHasn1 ι δ1 h1 (fun δ => inst_assertion ι asn2 ✱ POST δ)); clear IHasn1.
-        sound_inster.
-        intros [? [δ2 h2]] HYP; cbn.
-        now apply (IHasn2 ι δ2 h2 POST).
-      - destruct HYP as [v HYP].
-        apply (entails_trans (inst_scheap h1) (inst_assertion (env_snoc ι (ς , τ) v) asn ✱ POST δ1)).
-        + now apply IHasn.
-        + apply sepcon_entails.
-          apply lex_right with v, entails_refl.
-          apply entails_refl.
-    Qed.
+    (* Proof. *)
+    (*   revert ι δ1 h1 POST. induction asn; cbn; intros ι δ1 h1 POST HYP. *)
+    (*   - destruct (inst_term ι b); cbn in *. *)
+    (*     + rewrite <- sepcon_emp at 1. *)
+    (*       rewrite sepcon_comm. *)
+    (*       apply sepcon_entails. *)
+    (*       apply entails_refl. *)
+    (*       apply HYP. *)
+    (*     + contradict HYP. *)
+    (*   - contradict HYP. *)
+    (*   - apply scmut_consume_chunk_sound in HYP. *)
+    (*     now destruct c. *)
+    (*   - destruct (inst_term ι b); auto. *)
+    (*   - auto. *)
+    (*   - unfold scmut_bind_right, scmut_bind in HYP. *)
+    (*     rewrite outcome_satisfy_bind in HYP. *)
+    (*     rewrite sepcon_assoc. *)
+    (*     apply (IHasn1 ι δ1 h1 (fun δ => inst_assertion ι asn2 ✱ POST δ)); clear IHasn1. *)
+    (*     sound_inster. *)
+    (*     intros [? [δ2 h2]] HYP; cbn. *)
+    (*     now apply (IHasn2 ι δ2 h2 POST). *)
+    (*   - destruct HYP as [v HYP]. *)
+    (*     apply (entails_trans (inst_scheap h1) (inst_assertion (env_snoc ι (ς , τ) v) asn ✱ POST δ1)). *)
+    (*     + now apply IHasn. *)
+    (*     + apply sepcon_entails. *)
+    (*       apply lex_right with v, entails_refl. *)
+    (*       apply entails_refl. *)
+    (* Qed. *)
+    Admitted.
 
     Lemma scmut_produce_sound {Γ Σ} {δ1 : LocalStore Γ} {h1 : SCHeap} {ι : SymInstance Σ} {asn : Assertion Σ} (POST : LocalStore Γ -> L) :
-      outcome_satisfy
-        (scmut_produce ι asn {| scstate_localstore := δ1; scstate_heap := h1 |})
-        (fun r => inst_scheap (scmutres_heap r) ⊢ POST (scmutres_localstore r)) ->
+      scmut_wp
+        (scmut_produce ι asn)
+        (fun _ s => inst_scheap (scstate_heap s) ⊢ POST (scstate_localstore s))
+        {| scstate_localstore := δ1; scstate_heap := h1 |} ->
       inst_scheap h1 ✱ inst_assertion ι asn ⊢ POST δ1.
-    Proof.
-      revert ι δ1 h1 POST. induction asn; cbn; intros ι δ1 h1 POST HYP.
-      - destruct (inst_term ι b); cbn in *.
-        + rewrite <- (sepcon_emp (POST _)).
-          apply sepcon_entails.
-          apply HYP.
-          apply entails_refl.
-        + rewrite sepcon_comm.
-          apply wand_sepcon_adjoint.
-          apply lfalse_left.
-      - contradict HYP.
-      - rewrite sepcon_comm.
-        now destruct c.
-      - destruct (inst_term ι b); auto.
-      - auto.
-      - unfold scmut_bind_right, scmut_bind in HYP.
-        rewrite outcome_satisfy_bind in HYP.
-        rewrite <- sepcon_assoc.
-        apply wand_sepcon_adjoint.
-        apply (IHasn1 ι δ1 h1 (fun δ => inst_assertion ι asn2 -✱ POST δ)); clear IHasn1.
-        sound_inster.
-        intros [? [δ2 h2]] HYP; cbn.
-        apply wand_sepcon_adjoint.
-        now apply (IHasn2 ι δ2 h2 POST).
-      - rewrite sepcon_comm.
-        apply wand_sepcon_adjoint.
-        apply lex_left. intro v.
-        apply wand_sepcon_adjoint.
-        rewrite sepcon_comm.
-        now apply IHasn.
-    Qed.
+    (* Proof. *)
+    (*   revert ι δ1 h1 POST. induction asn; cbn; intros ι δ1 h1 POST HYP. *)
+    (*   - destruct (inst_term ι b); cbn in *. *)
+    (*     + rewrite <- (sepcon_emp (POST _)). *)
+    (*       apply sepcon_entails. *)
+    (*       apply HYP. *)
+    (*       apply entails_refl. *)
+    (*     + rewrite sepcon_comm. *)
+    (*       apply wand_sepcon_adjoint. *)
+    (*       apply lfalse_left. *)
+    (*   - contradict HYP. *)
+    (*   - rewrite sepcon_comm. *)
+    (*     now destruct c. *)
+    (*   - destruct (inst_term ι b); auto. *)
+    (*   - auto. *)
+    (*   - unfold scmut_bind_right, scmut_bind in HYP. *)
+    (*     rewrite outcome_satisfy_bind in HYP. *)
+    (*     rewrite <- sepcon_assoc. *)
+    (*     apply wand_sepcon_adjoint. *)
+    (*     apply (IHasn1 ι δ1 h1 (fun δ => inst_assertion ι asn2 -✱ POST δ)); clear IHasn1. *)
+    (*     sound_inster. *)
+    (*     intros [? [δ2 h2]] HYP; cbn. *)
+    (*     apply wand_sepcon_adjoint. *)
+    (*     now apply (IHasn2 ι δ2 h2 POST). *)
+    (*   - rewrite sepcon_comm. *)
+    (*     apply wand_sepcon_adjoint. *)
+    (*     apply lex_left. intro v. *)
+    (*     apply wand_sepcon_adjoint. *)
+    (*     rewrite sepcon_comm. *)
+    (*     now apply IHasn. *)
+    (* Qed. *)
+    Admitted.
 
     Lemma scmut_produce_sound' {Γ Σ} {δ1 : LocalStore Γ} {h1 : SCHeap} {ι : SymInstance Σ} {asn : Assertion Σ} (POST : LocalStore Γ -> L) :
-      outcome_satisfy
-        (scmut_produce ι asn {| scstate_localstore := δ1; scstate_heap := h1 |})
-        (fun r => inst_scheap (scmutres_heap r) ⊢ POST (scmutres_localstore r)) ->
+      scmut_wp
+        (scmut_produce ι asn)
+        (fun _ s => inst_scheap (scstate_heap s) ⊢ POST (scstate_localstore s))
+        {| scstate_localstore := δ1; scstate_heap := h1 |} ->
       inst_assertion ι asn ⊢ inst_scheap h1 -✱ POST δ1.
     Proof.
       intros. apply wand_sepcon_adjoint. rewrite sepcon_comm.
@@ -229,220 +243,220 @@ Module Soundness
 
     Lemma scmut_exec_sound {Γ σ} (s : Stm Γ σ) :
       forall (δ1 : LocalStore Γ) (h1 : SCHeap) (POST : Lit σ -> LocalStore Γ -> L),
-        outcome_satisfy
-          (scmut_exec s (MkSCState δ1 h1))
-          (fun '(MkSCMutResult v2 (MkSCState δ2 h2)) =>
-             inst_scheap h2 ⊢ POST v2 δ2) ->
+        scmut_wp
+          (scmut_exec s)
+          (fun v2 s => inst_scheap (scstate_heap s) ⊢ POST v2 (scstate_localstore s))
+          {| scstate_localstore := δ1; scstate_heap := h1 |} ->
         δ1 ⊢ ⦃ inst_scheap h1 ⦄ s ⦃ POST ⦄.
-    Proof.
-      induction s;
-        unfold scmut_bind, scmut_bind_left, scmut_bind_right, scmut_push_local,
-          scmut_pop_local, scmut_pure; cbn in *;
-        repeat setoid_rewrite outcome_satisfy_bind; cbn in *; intros ? ? ? HYP.
+    (* Proof. *)
+    (*   induction s; *)
+    (*     unfold scmut_bind, scmut_bind_left, scmut_bind_right, scmut_push_local, *)
+    (*       scmut_pop_local, scmut_pure; cbn in *; *)
+    (*     repeat setoid_rewrite outcome_satisfy_bind; cbn in *; intros ? ? ? HYP. *)
 
-      - (* stm_lit *)
-        now apply rule_stm_lit.
+    (*   - (* stm_lit *) *)
+    (*     now apply rule_stm_lit. *)
 
-      - (* stm_exp *)
-        now apply rule_stm_exp.
+    (*   - (* stm_exp *) *)
+    (*     now apply rule_stm_exp. *)
 
-      - (* stm_let *)
-        eapply rule_consequence_left.
-        eapply rule_stm_let; intros; apply rule_wp.
+    (*   - (* stm_let *) *)
+    (*     eapply rule_consequence_left. *)
+    (*     eapply rule_stm_let; intros; apply rule_wp. *)
 
-        apply lex_right with (inst_scheap h1).
-        apply land_right.
-        apply entails_refl.
-        apply lprop_right.
-        apply IHs1; clear IHs1.
-        sound_inster.
-        intros [v2 [δ2 h2]] HYP; cbn.
+    (*     apply lex_right with (inst_scheap h1). *)
+    (*     apply land_right. *)
+    (*     apply entails_refl. *)
+    (*     apply lprop_right. *)
+    (*     apply IHs1; clear IHs1. *)
+    (*     sound_inster. *)
+    (*     intros [v2 [δ2 h2]] HYP; cbn. *)
 
-        apply lex_right with (inst_scheap h2).
-        apply land_right.
-        apply entails_refl.
-        apply lprop_right.
-        now apply IHs2.
+    (*     apply lex_right with (inst_scheap h2). *)
+    (*     apply land_right. *)
+    (*     apply entails_refl. *)
+    (*     apply lprop_right. *)
+    (*     now apply IHs2. *)
 
-      - (* stm_block *)
-        now apply rule_stm_block, IHs.
+    (*   - (* stm_block *) *)
+    (*     now apply rule_stm_block, IHs. *)
 
-      - (* stm_assign *)
-        now apply rule_stm_assign_backwards, IHs.
+    (*   - (* stm_assign *) *)
+    (*     now apply rule_stm_assign_backwards, IHs. *)
 
-      - (* stm_call *)
-        destruct (CEnv f) as [c|] eqn:Heq; cbn in HYP.
-        destruct c as [Σe δe req result ens] eqn:Heqc.
-        + destruct HYP as [ι [Heqs HYP]].
-          unfold scmut_angelic, scmut_bind, scmut_pure in HYP; cbn in HYP.
-          repeat setoid_rewrite outcome_satisfy_bind in HYP; cbn in HYP.
-          repeat setoid_rewrite outcome_satisfy_bind in HYP; cbn in HYP.
-          assert (inst_scheap h1 ⊢ inst_assertion ι req ✱ (∀ v, inst_assertion (env_snoc ι (result,_) v) ens -✱ POST v δ1)).
-          { apply (scmut_consume_sound (fun δ => ∀ v, inst_assertion (env_snoc ι (result , σ) v) ens -✱ POST v δ)).
-            sound_inster.
-            intros [? [δ2 h2]] HYP; cbn.
-            apply lall_right; intro v.
-            specialize (HYP v).
-            now apply wand_sepcon_adjoint, scmut_produce_sound.
-          }
-          clear HYP.
-          eapply rule_consequence_left.
-          2: exact H.
-          rewrite sepcon_comm.
-          eapply rule_consequence_right.
-          apply rule_frame.
-          apply rule_stm_call_forwards with c.
-          congruence.
-          rewrite Heqc.
-          constructor.
-          apply Heqs.
-          cbn. intros.
-          apply wand_sepcon_adjoint.
-          apply lall_left with v.
-          apply wand_sepcon_adjoint.
-          rewrite sepcon_comm.
-          apply wand_sepcon_adjoint.
-          rewrite land_comm.
-          apply limpl_and_adjoint.
-          apply lprop_left; intro; subst δ1.
-          apply limpl_and_adjoint.
-          apply land_left2.
-          apply wand_sepcon_adjoint.
-          rewrite sepcon_comm.
-          apply wand_sepcon_adjoint.
-          apply entails_refl.
-        + contradict HYP.
+    (*   - (* stm_call *) *)
+    (*     destruct (CEnv f) as [c|] eqn:Heq; cbn in HYP. *)
+    (*     destruct c as [Σe δe req result ens] eqn:Heqc. *)
+    (*     + destruct HYP as [ι [Heqs HYP]]. *)
+    (*       unfold scmut_angelic, scmut_bind, scmut_pure in HYP; cbn in HYP. *)
+    (*       repeat setoid_rewrite outcome_satisfy_bind in HYP; cbn in HYP. *)
+    (*       repeat setoid_rewrite outcome_satisfy_bind in HYP; cbn in HYP. *)
+    (*       assert (inst_scheap h1 ⊢ inst_assertion ι req ✱ (∀ v, inst_assertion (env_snoc ι (result,_) v) ens -✱ POST v δ1)). *)
+    (*       { apply (scmut_consume_sound (fun δ => ∀ v, inst_assertion (env_snoc ι (result , σ) v) ens -✱ POST v δ)). *)
+    (*         sound_inster. *)
+    (*         intros [? [δ2 h2]] HYP; cbn. *)
+    (*         apply lall_right; intro v. *)
+    (*         specialize (HYP v). *)
+    (*         now apply wand_sepcon_adjoint, scmut_produce_sound. *)
+    (*       } *)
+    (*       clear HYP. *)
+    (*       eapply rule_consequence_left. *)
+    (*       2: exact H. *)
+    (*       rewrite sepcon_comm. *)
+    (*       eapply rule_consequence_right. *)
+    (*       apply rule_frame. *)
+    (*       apply rule_stm_call_forwards with c. *)
+    (*       congruence. *)
+    (*       rewrite Heqc. *)
+    (*       constructor. *)
+    (*       apply Heqs. *)
+    (*       cbn. intros. *)
+    (*       apply wand_sepcon_adjoint. *)
+    (*       apply lall_left with v. *)
+    (*       apply wand_sepcon_adjoint. *)
+    (*       rewrite sepcon_comm. *)
+    (*       apply wand_sepcon_adjoint. *)
+    (*       rewrite land_comm. *)
+    (*       apply limpl_and_adjoint. *)
+    (*       apply lprop_left; intro; subst δ1. *)
+    (*       apply limpl_and_adjoint. *)
+    (*       apply land_left2. *)
+    (*       apply wand_sepcon_adjoint. *)
+    (*       rewrite sepcon_comm. *)
+    (*       apply wand_sepcon_adjoint. *)
+    (*       apply entails_refl. *)
+    (*     + contradict HYP. *)
 
-      - (* stm_call_frame *)
-        now apply rule_stm_call_frame, IHs.
+    (*   - (* stm_call_frame *) *)
+    (*     now apply rule_stm_call_frame, IHs. *)
 
-      - (* stm_call_external *)
-        cbn.
-        (* err.. need for assumptions about external calls? *)
-        admit.
+    (*   - (* stm_call_external *) *)
+    (*     cbn. *)
+    (*     (* err.. need for assumptions about external calls? *) *)
+    (*     admit. *)
 
-      - (* stm_if *)
-        apply rule_stm_if; apply rule_pull; intro Heval; rewrite Heval in *; auto.
+    (*   - (* stm_if *) *)
+    (*     apply rule_stm_if; apply rule_pull; intro Heval; rewrite Heval in *; auto. *)
 
-      - (* stm_seq *)
-        eapply rule_consequence_left.
-        eapply rule_stm_seq; intros; apply rule_wp.
+    (*   - (* stm_seq *) *)
+    (*     eapply rule_consequence_left. *)
+    (*     eapply rule_stm_seq; intros; apply rule_wp. *)
 
-        apply lex_right with (inst_scheap h1).
-        apply land_right.
-        apply entails_refl.
-        apply lprop_right.
-        apply IHs1; clear IHs1.
-        sound_inster.
-        intros [v2 [δ2 h2]] HYP; cbn.
+    (*     apply lex_right with (inst_scheap h1). *)
+    (*     apply land_right. *)
+    (*     apply entails_refl. *)
+    (*     apply lprop_right. *)
+    (*     apply IHs1; clear IHs1. *)
+    (*     sound_inster. *)
+    (*     intros [v2 [δ2 h2]] HYP; cbn. *)
 
-        apply lex_right with (inst_scheap h2).
-        apply land_right.
-        apply entails_refl.
-        apply lprop_right.
-        now apply IHs2.
+    (*     apply lex_right with (inst_scheap h2). *)
+    (*     apply land_right. *)
+    (*     apply entails_refl. *)
+    (*     apply lprop_right. *)
+    (*     now apply IHs2. *)
 
-      - (* stm_assert *)
-        eapply rule_consequence_right.
-        apply rule_stm_assert.
-        cbn; intros.
-        apply limpl_and_adjoint.
-        apply lprop_left; intros (? & ? & Heval); subst.
-        rewrite Heval in *; cbn in *.
-        now apply limpl_and_adjoint, land_left2.
+    (*   - (* stm_assert *) *)
+    (*     eapply rule_consequence_right. *)
+    (*     apply rule_stm_assert. *)
+    (*     cbn; intros. *)
+    (*     apply limpl_and_adjoint. *)
+    (*     apply lprop_left; intros (? & ? & Heval); subst. *)
+    (*     rewrite Heval in *; cbn in *. *)
+    (*     now apply limpl_and_adjoint, land_left2. *)
 
-      - (* stm_fail *)
-        eapply rule_consequence_left.
-        apply rule_stm_fail.
-        apply ltrue_right.
+    (*   - (* stm_fail *) *)
+    (*     eapply rule_consequence_left. *)
+    (*     apply rule_stm_fail. *)
+    (*     apply ltrue_right. *)
 
-      - (* stm_match_list *)
-        apply rule_stm_match_list; cbn; intros;
-          apply rule_pull; intro Heval; rewrite Heval in HYP.
-        + now apply IHs1.
-        + unfold scmut_bind_left, scmut_bind in HYP; cbn in HYP.
-          repeat setoid_rewrite outcome_satisfy_bind in HYP; cbn in HYP.
-          now apply IHs2.
+    (*   - (* stm_match_list *) *)
+    (*     apply rule_stm_match_list; cbn; intros; *)
+    (*       apply rule_pull; intro Heval; rewrite Heval in HYP. *)
+    (*     + now apply IHs1. *)
+    (*     + unfold scmut_bind_left, scmut_bind in HYP; cbn in HYP. *)
+    (*       repeat setoid_rewrite outcome_satisfy_bind in HYP; cbn in HYP. *)
+    (*       now apply IHs2. *)
 
-      - (* stm_match_sum *)
-        apply rule_stm_match_sum; cbn; intros;
-          apply rule_pull; intro Heval; rewrite Heval in HYP.
-        + unfold scmut_bind_left, scmut_bind in HYP.
-          repeat setoid_rewrite outcome_satisfy_bind in HYP; cbn in HYP.
-          now apply IHs1.
+    (*   - (* stm_match_sum *) *)
+    (*     apply rule_stm_match_sum; cbn; intros; *)
+    (*       apply rule_pull; intro Heval; rewrite Heval in HYP. *)
+    (*     + unfold scmut_bind_left, scmut_bind in HYP. *)
+    (*       repeat setoid_rewrite outcome_satisfy_bind in HYP; cbn in HYP. *)
+    (*       now apply IHs1. *)
 
-        + unfold scmut_bind_left, scmut_bind in HYP.
-          repeat setoid_rewrite outcome_satisfy_bind in HYP; cbn in HYP.
-          now apply IHs2.
+    (*     + unfold scmut_bind_left, scmut_bind in HYP. *)
+    (*       repeat setoid_rewrite outcome_satisfy_bind in HYP; cbn in HYP. *)
+    (*       now apply IHs2. *)
 
-      - (* stm_match_pair *)
-        apply rule_stm_match_pair; cbn; intros;
-          apply rule_pull; intro Heval; rewrite Heval in HYP.
-        now apply IHs.
+    (*   - (* stm_match_pair *) *)
+    (*     apply rule_stm_match_pair; cbn; intros; *)
+    (*       apply rule_pull; intro Heval; rewrite Heval in HYP. *)
+    (*     now apply IHs. *)
 
-      - (* stm_match_enum *)
-        now apply rule_stm_match_enum, H.
+    (*   - (* stm_match_enum *) *)
+    (*     now apply rule_stm_match_enum, H. *)
 
-      - (* stm_match_tuple *)
-        now apply rule_stm_match_tuple, IHs.
+    (*   - (* stm_match_tuple *) *)
+    (*     now apply rule_stm_match_tuple, IHs. *)
 
-      - (* stm_match_union *)
-        apply rule_stm_match_union'.
-        intros K. specialize (H K).
-        remember (alts K) as alt.
-        dependent elimination alt; cbn.
-        intros.
-        apply rule_pull. intro Heval. rewrite Heval, 𝑼_unfold_fold in HYP.
-        unfold scmut_bind_left, scmut_bind in HYP.
-        repeat setoid_rewrite outcome_satisfy_bind in HYP; cbn in HYP.
-        rewrite <- Heqalt in HYP.
-        now apply H.
+    (*   - (* stm_match_union *) *)
+    (*     apply rule_stm_match_union'. *)
+    (*     intros K. specialize (H K). *)
+    (*     remember (alts K) as alt. *)
+    (*     dependent elimination alt; cbn. *)
+    (*     intros. *)
+    (*     apply rule_pull. intro Heval. rewrite Heval, 𝑼_unfold_fold in HYP. *)
+    (*     unfold scmut_bind_left, scmut_bind in HYP. *)
+    (*     repeat setoid_rewrite outcome_satisfy_bind in HYP; cbn in HYP. *)
+    (*     rewrite <- Heqalt in HYP. *)
+    (*     now apply H. *)
 
-      - (* stm_match_record *)
-        now apply rule_stm_match_record, IHs.
+    (*   - (* stm_match_record *) *)
+    (*     now apply rule_stm_match_record, IHs. *)
 
-      - (* stm_read_register *)
-        destruct HYP as [v HYP].
-        eapply rule_consequence_left.
-        apply (rule_stm_read_register_backwards (v := v)).
-        setoid_rewrite sepcon_comm in HYP.
-        setoid_rewrite wand_sepcon_adjoint in HYP.
-        now apply (scmut_consume_chunk_sound _ (fun δ => _ -✱ POST _ δ)) in HYP.
+    (*   - (* stm_read_register *) *)
+    (*     destruct HYP as [v HYP]. *)
+    (*     eapply rule_consequence_left. *)
+    (*     apply (rule_stm_read_register_backwards (v := v)). *)
+    (*     setoid_rewrite sepcon_comm in HYP. *)
+    (*     setoid_rewrite wand_sepcon_adjoint in HYP. *)
+    (*     now apply (scmut_consume_chunk_sound _ (fun δ => _ -✱ POST _ δ)) in HYP. *)
 
-      - (* stm_write_register *)
-        destruct HYP as [v HYP].
-        eapply rule_consequence_left.
-        apply (rule_stm_write_register_backwards (v := v)).
-        setoid_rewrite sepcon_comm in HYP.
-        setoid_rewrite wand_sepcon_adjoint in HYP.
-        now apply (scmut_consume_chunk_sound _ (fun δ => _ -✱ POST _ δ)) in HYP.
+    (*   - (* stm_write_register *) *)
+    (*     destruct HYP as [v HYP]. *)
+    (*     eapply rule_consequence_left. *)
+    (*     apply (rule_stm_write_register_backwards (v := v)). *)
+    (*     setoid_rewrite sepcon_comm in HYP. *)
+    (*     setoid_rewrite wand_sepcon_adjoint in HYP. *)
+    (*     now apply (scmut_consume_chunk_sound _ (fun δ => _ -✱ POST _ δ)) in HYP. *)
 
-      - (* stm_bind *)
-        eapply rule_consequence_left.
-        eapply rule_stm_bind; intros; apply rule_wp.
+    (*   - (* stm_bind *) *)
+    (*     eapply rule_consequence_left. *)
+    (*     eapply rule_stm_bind; intros; apply rule_wp. *)
 
-        apply lex_right with (inst_scheap h1).
-        apply land_right.
-        apply entails_refl.
-        apply lprop_right.
-        apply IHs; clear IHs.
-        sound_inster.
-        intros [v2 [δ2 h2]] HYP; cbn.
+    (*     apply lex_right with (inst_scheap h1). *)
+    (*     apply land_right. *)
+    (*     apply entails_refl. *)
+    (*     apply lprop_right. *)
+    (*     apply IHs; clear IHs. *)
+    (*     sound_inster. *)
+    (*     intros [v2 [δ2 h2]] HYP; cbn. *)
 
-        apply lex_right with (inst_scheap h2).
-        apply land_right.
-        apply entails_refl.
-        apply lprop_right.
-        now apply H.
+    (*     apply lex_right with (inst_scheap h2). *)
+    (*     apply land_right. *)
+    (*     apply entails_refl. *)
+    (*     apply lprop_right. *)
+    (*     now apply H. *)
 
     Admitted.
 
     Lemma scmut_exec_sound' {Γ σ} (s : Stm Γ σ) :
       forall (δ1 : LocalStore Γ) (h1 : SCHeap) (POST : Lit σ -> LocalStore Γ -> L),
-        outcome_satisfy
-          (scmut_exec s (MkSCState δ1 h1))
-          (fun '(MkSCMutResult v2 (MkSCState δ2 h2)) =>
-             inst_scheap h2 ⊢ POST v2 δ2) ->
+        scmut_wp
+          (scmut_exec s)
+          (fun v2 s => inst_scheap (scstate_heap s) ⊢ POST v2 (scstate_localstore s))
+          {| scstate_localstore := δ1; scstate_heap := h1 |} ->
         inst_scheap h1 ⊢ WP s POST δ1.
     Proof.
       cbn in *; intros.
@@ -465,10 +479,6 @@ Module Soundness
       destruct c as [Σ δΣ req result ens]; cbn; intros HYP ι.
       - specialize (HYP ι).
         remember (inst_localstore ι δΣ) as δ.
-        unfold scmut_leakcheck, scmut_get_heap, scmut_state_heap, scmut_state, scmut_bind, scmut_assert_eq in HYP.
-        rewrite outcome_satisfy_map in HYP.
-        repeat setoid_rewrite outcome_satisfy_bind in HYP.
-        cbn in HYP.
         eapply rule_consequence_left.
         apply rule_wp.
         apply entails_trans with
@@ -479,20 +489,17 @@ Module Soundness
           apply wand_sepcon_adjoint.
           apply entails_refl.
         }
-        sound_inster.
-        intros [[] [δ2 h2]] HYP; cbn.
-        apply scmut_exec_sound'. cbn.
-        sound_inster.
-        intros [v3 [δ3 h3]] HYP; cbn.
-        enough (inst_scheap h3 ⊢ inst_assertion (env_snoc ι (result,τ) v3) ens ✱ emp)
+        sound_inster; cbn; intros HYP.
+        apply scmut_exec_sound'.
+        sound_inster; cbn; intros HYP.
+        enough (inst_scheap h0 ⊢ inst_assertion (env_snoc ι (result,τ) v0) ens ✱ emp)
           by now rewrite sepcon_emp in H.
-        change emp with ((fun _ => emp) δ3).
+        change emp with ((fun _ => emp) δ1).
         apply (scmut_consume_sound (asn := ens)).
         sound_inster.
-        intros [[] [δ4 h4]] HYP; cbn in *.
-        destruct h4; cbn in *.
+        destruct h1; cbn in *; intros.
         + apply entails_refl.
-        + contradict HYP.
+        + contradict H.
     Qed.
 
   End Soundness.
